Sequence of main games for PSS, with some of the intermediate statements.

examples/PSS.ec
@@ -4,6 +4,7 @@ require import Real.
 require import FSet.
 require import Map.
 require import Pair.
+require import Distr.
 
 (*** General definitions *)
 (** Lengths *)
@@ -27,6 +28,15 @@ lemma leq0_kg2: 0 <= kg2 by [].
 
 op k':int = k - 1.
 lemma leq0_k': 0 <= k' by [].
+
+op qS:int.
+axiom leq0_qS: 0 <= qS.
+
+op qH:int.
+axiom leq0_qH: 0 <= qH.
+
+op qG:int.
+axiom leq0_qG: 0 <= qG.
 
 (** Types *)
 require AWord.
@@ -70,7 +80,7 @@ clone import AWord as G2Tag with
   op length = kg2.
 
 (* Domain of RSA *)
-op sample_plain: signature distr. (* Whereby we sample only with the first byte/bit set to 0 *)
+op sample_plain: signature distr.
 
 (** Instantiating *)
 require PKS.
@@ -80,13 +90,16 @@ require RandomOracle.
 clone import OW as RSA with
   type t <- signature,
   op sample_t <- sample_plain,
-  op f_dom = (lambda (pk:pkey) (x:signature), cpTrue x),
-  op f_rng = (lambda (pk:pkey) (x:signature), cpTrue x),
-  op finv_dom = (lambda (sk:skey) (x:signature), cpTrue x),
-  op finv_rng = (lambda (sk:skey) (x:signature), cpTrue x)
+  op f_dom = (lambda (pk:pkey) (x:signature), true),
+  op f_rng = (lambda (pk:pkey) (x:signature), true),
+  op finv_dom = (lambda (sk:skey) (x:signature), true),
+  op finv_rng = (lambda (sk:skey) (x:signature), true)
   proof f_rng_sub_finv_dom by smt,
         finv_rng_sub_f_dom by smt,
         f_dom_sample_t by smt.
+
+op ( * ): signature -> signature -> pkey -> signature.
+axiom homo_f_mul (x y:signature) pk: f pk ((x * y) pk) = (f pk x * f pk y) pk.
 
 clone import RandomOracle as Gt with
   type from <- htag,
@@ -95,7 +108,7 @@ clone import RandomOracle as Gt with
 module G = Gt.ROM.RO.
 
 clone import RandomOracle as Ht with
-  type from <- message,
+  type from <- (message * salt),
   type to <- htag,
   op dsample <- sample_htag.
 module H = Ht.ROM.RO.
@@ -143,7 +156,7 @@ module PSS(G:Gt.Oracle,H:Ht.Oracle): Scheme = {
     var y:signature;
 
     r = $sample_salt;
-    w  = H.o(m || (to_bits r));
+    w  = H.o((m,r));
     rMask  = g1(w);
     maskedR = rMask ^ r;
     gamma  = g2(w);
@@ -170,7 +183,7 @@ module PSS(G:Gt.Oracle,H:Ht.Oracle): Scheme = {
     gamma = G2Tag.from_bits (sub (to_bits y) (k1 + k0 + 1) kg2);
     rMask  = g1(w);
     r = rMask ^ maskedR;
-    w'  = H.o(m || to_bits r);
+    w'  = H.o((m,r));
     gamma'  = g2(w);
     return (w = w' /\ gamma = gamma' /\ !b);
   }
@@ -181,14 +194,28 @@ module type CMA_2RO(G:Gt.ARO,H:Ht.ARO,S:AdvOracles) = {
   fun forge(pk:pkey): message * signature
 }.
 
-(** First transition: Folding in two calls to G, inlining *)
+(** Inlining the oracles that do not get modified much *)
 module type PartialOracles = {
   fun init(): pkey
   fun sign(m:message): signature
   fun fresh(m:message): bool
 }.
 
-module G0o(G:Gt.Oracle,H:Ht.Oracle): PartialOracles = {
+module Mem = {
+  var pk:pkey
+  var sk:skey
+  var n:int
+  var xstar:signature
+
+  fun init(pk:pkey,sk:skey): unit = {
+    Mem.pk = pk;
+    Mem.sk = sk;
+    n = 3; (* Use the public key's modulus *)
+    xstar = $sample_plain;
+  }
+}.
+
+module SGen(H:Ht.Oracle): PartialOracles = {
   var pk:pkey
   var sk:skey
 
@@ -199,391 +226,7 @@ module G0o(G:Gt.Oracle,H:Ht.Oracle): PartialOracles = {
     H.init();
     qs = FSet.empty;
     (pk,sk) = $keypairs;
-    return pk;
-  }
-
-  fun sign(m:message): signature = {
-    var r:salt;
-    var g:gtag;
-    var rMask:salt;
-    var maskedR:salt;
-    var w:htag;
-    var gamma:g2tag;
-    var y:signature;
-
-    qs = add m qs;
-    r = $sample_salt;
-    w  = H.o(m || (to_bits r));
-    g = G.o(w);
-    rMask  = Salt.from_bits (sub (to_bits g) 0 k0);
-    maskedR = rMask ^ r;
-    gamma  = G2Tag.from_bits (sub (to_bits g) k0 kg2);
-    y = Signature.from_bits (zeros 1 || (to_bits w) || (to_bits maskedR) || (to_bits gamma));
-    return finv sk y;
-  } 
-
-  fun fresh(m:message): bool = {
-    return !mem m qs;
-  }
-}.
-
-module G0(G:Gt.Oracle,H:Ht.Oracle,O:PartialOracles,A:AdvCMA) = {
-  module A = A(O)
-
-  fun main(): bool = {
-    var pk:pkey;
-    var m:message;
-    var s:signature;
-    var y:signature;
-    var w:htag;
-    var w':htag;
-    var g:gtag;
-    var maskedR:salt;
-    var gamma:g2tag;
-    var gamma':g2tag;
-    var rMask:salt;
-    var r:salt;
-    var forged, fresh:bool;
-
-    pk = O.init();
-    (m,s) = A.forge(pk);
-
-    y = (f pk s);
-    forged = (sub (to_bits y) 0 1 <> zeros 1);
-    w = HTag.from_bits (sub (to_bits y) 1 k1);
-    maskedR = Salt.from_bits (sub (to_bits y) (k1 + 1) k0);
-    gamma = G2Tag.from_bits (sub (to_bits y) (k1 + k0 + 1) kg2);
-    g = G.o(w);
-    rMask  = Salt.from_bits (sub (to_bits g) 0 k0);
-    r = rMask ^ maskedR;
-    w'  = H.o(m || to_bits r);
-    gamma'  = G2Tag.from_bits (sub (to_bits g) k0 kg2);
-    forged =  w = w' /\ gamma = gamma' /\ !forged;
-
-    fresh = O.fresh(m);
-    return forged /\ fresh;
-  }
-}.
-
-section.
-declare module Adv:CMA_2RO {Wrap,PSS,Gt.ROM.RO,Ht.ROM.RO,G0,G0o}.
-axiom AdvL (G<:Gt.Oracle) (H<:Ht.Oracle):
-  islossless G.o => islossless H.o =>
-  islossless Adv(G,H,Wrap(PSS(G,H))).forge.
-
-(* Proving semantic equivalence: both random oracles can be kept abstract,
-   although we need to know that successive calls to G with the same argument
-   return the same result. *)
-section.
-declare module G:Gt.Oracle {Adv,Wrap,G0o,G0}.
-axiom correct_G: mu sample_gtag cpTrue = 1%r =>
-  equiv [Gt.Correct(G).call2 ~ Gt.Correct(G).call1: ={glob G, x} ==> ={glob G} /\ res{1} = (res,res){2}].
-local module CorrectG = Gt.Correct(G).
-
-declare module H:Ht.Oracle {Adv,Wrap,G,G0o,G0}.
-
-(* Folding in the two calls to G *)
-local module PSS'(G:Gt.Oracle,H:Ht.Oracle): Scheme = {
-  fun init(): unit = {
-    G.init();
-    H.init();
-  }
-
-  fun keygen():(pkey * skey) = {
-    var (pk, sk):(pkey * skey);
-    (pk,sk) = $keypairs;
-    return (pk,sk);
-  }
-
-  fun sign(sk:skey, m:message):signature = {
-    var r:salt;
-    var g,g':gtag;
-    var rMask:salt;
-    var maskedR:salt;
-    var w:htag;
-    var gamma:g2tag;
-    var y:signature;
-
-    r = $sample_salt;
-    w  = H.o(m || (to_bits r));
-    (g,g') = CorrectG.call2(w);
-    rMask = Salt.from_bits (sub (to_bits g) 0 k0);
-    maskedR = rMask ^ r;
-    gamma  = G2Tag.from_bits (sub (to_bits g') k0 kg2);
-    y = Signature.from_bits (zeros 1 || (to_bits w) || (to_bits maskedR) || (to_bits gamma));
-    return (finv sk y);
-  }
-
-  fun verify(pk:pkey, m:message, s:signature):bool = {
-    var y:signature;
-    var g, g':gtag;
-    var w:htag;
-    var w':htag;
-    var maskedR:salt;
-    var gamma:g2tag;
-    var gamma':g2tag;
-    var rMask:salt;
-    var r:salt;
-    var b:bool;
-
-    y = (f pk s);
-    b = (sub (to_bits y) 0 1 <> zeros 1);
-    w = HTag.from_bits (sub (to_bits y) 1 k1);
-    maskedR = Salt.from_bits (sub (to_bits y) (k1 + 1) k0);
-    gamma = G2Tag.from_bits (sub (to_bits y) (k1 + k0 + 1) kg2);
-    (g,g') = CorrectG.call2(w);
-    rMask  = Salt.from_bits (sub (to_bits g) 0 k0);
-    r = rMask ^ maskedR;
-    w'  = H.o(m || to_bits r);
-    gamma'  = G2Tag.from_bits (sub (to_bits g') k0 kg2);
-    return (w = w' /\ gamma = gamma' /\ !b);
-  }
-}.
-
-local equiv PSS_PSS':
-  EF_CMA(Wrap(PSS(G,H)),Adv(G,H)).main ~ EF_CMA(Wrap(PSS'(G,H)),Adv(G,H)).main:
-  ={glob Adv} ==> ={res}.
-proof.
-fun.
-call (_: ={Wrap.qs, m} ==> ={res});
-  first by fun; wp.
-call (_: ={glob H, glob G, Wrap.pk, m, s} ==> ={res});
-  first by fun; call (_: ={glob H, glob G, Wrap.pk, pk, m, s} ==> ={res})=> //;
-             fun; inline PSS(G,H).g1 PSS(G,H).g2 CorrectG.call2;
-                  swap{1} 11 -4; swap{1} 12 -3; eqobs_in; wp; eqobs_in.
-call (_: ={glob H, glob G, glob Wrap}).
-  fun; call (_: ={glob H, glob G, Wrap.sk, sk, m} ==> ={glob H, glob G, Wrap.sk, res});
-    last by wp.
-    fun; inline PSS(G,H).g1 PSS(G,H).g2 CorrectG.call2;
-         swap{1} 7 -3; swap{1} 8 -2; eqobs_in; wp; eqobs_in.
-  by fun (={glob G, glob Wrap}).
-  by fun (={glob H, glob Wrap}).
-call (_: true ==> ={glob H, glob G, glob Wrap, res})=> //.
-  by fun; eqobs_in.
-qed.
-
-local module PSS''(G:Gt.Oracle,H:Ht.Oracle): Scheme = {
-  fun init(): unit = {
-    G.init();
-    H.init();
-  }
-
-  fun keygen():(pkey * skey) = {
-    var (pk, sk):(pkey * skey);
-    (pk,sk) = $keypairs;
-    return (pk,sk);
-  }
-
-  fun sign(sk:skey, m:message):signature = {
-    var r:salt;
-    var g:gtag;
-    var rMask:salt;
-    var maskedR:salt;
-    var w:htag;
-    var gamma:g2tag;
-    var y:signature;
-
-    r = $sample_salt;
-    w  = H.o(m || (to_bits r));
-    g = CorrectG.call1(w);
-    rMask = Salt.from_bits (sub (to_bits g) 0 k0);
-    maskedR = rMask ^ r;
-    gamma  = G2Tag.from_bits (sub (to_bits g) k0 kg2);
-    y = Signature.from_bits (zeros 1 || (to_bits w) || (to_bits maskedR) || (to_bits gamma));
-    return (finv sk y);
-  }
-
-  fun verify(pk:pkey, m:message, s:signature):bool = {
-    var y:signature;
-    var g:gtag;
-    var w:htag;
-    var w':htag;
-    var maskedR:salt;
-    var gamma:g2tag;
-    var gamma':g2tag;
-    var rMask:salt;
-    var r:salt;
-    var b:bool;
-
-    y = (f pk s);
-    b = (sub (to_bits y) 0 1 <> zeros 1);
-    w = HTag.from_bits (sub (to_bits y) 1 k1);
-    maskedR = Salt.from_bits (sub (to_bits y) (k1 + 1) k0);
-    gamma = G2Tag.from_bits (sub (to_bits y) (k1 + k0 + 1) kg2);
-    g = CorrectG.call1(w);
-    rMask  = Salt.from_bits (sub (to_bits g) 0 k0);
-    r = rMask ^ maskedR;
-    w'  = H.o(m || to_bits r);
-    gamma'  = G2Tag.from_bits (sub (to_bits g) k0 kg2);
-    return (w = w' /\ gamma = gamma' /\ !b);
-  }
-}.
-
-local equiv PSS'_PSS'':
-  EF_CMA(Wrap(PSS'(G,H)),Adv(G,H)).main ~ EF_CMA(Wrap(PSS''(G,H)),Adv(G,H)).main:
-  ={glob Adv} ==> ={res}.
-proof.
-fun;
-call (_: ={Wrap.qs, m} ==> ={res});
-  first by fun; wp.
-call (_: ={glob H, glob G, Wrap.pk, m, s} ==> ={res});
-  first by fun; call (_: ={glob H, glob G, Wrap.pk, pk, m, s} ==> ={res})=> //;
-             fun; eqobs_in; (call (correct_G _); first by apply gtagL); wp.
-call (_: ={glob H, glob G, glob Wrap}).
-  fun; call (_: ={glob H, glob G, Wrap.sk, sk, m} ==> ={glob H, glob G, Wrap.sk, res});
-    last by wp.
-    fun; eqobs_in; (call (correct_G _); first by apply gtagL); wp;
-    call (_: ={glob H, x} ==> ={glob H, res});
-      first by fun (true).
-    by rnd.
-  by fun (={glob G, glob Wrap}).
-  by fun (={glob H, glob Wrap}).
-call (_: true ==> ={glob H, glob G, glob Wrap, res})=> //;
-  by fun; eqobs_in.
-qed.
-
-(** Back to the real proof *)
-local lemma PSS''_G0_fresh:
-  equiv [Wrap(PSS''(G,H)).fresh ~ G0o(G,H).fresh: ={m} /\ Wrap.qs{1} = G0o.qs{2} ==> ={res}]
-by by fun.
-
-local lemma PSS''_G0_sign:
-  equiv [Wrap(PSS''(G,H)).sign ~ G0o(G,H).sign:
-    ={m,glob G, glob H} /\ Wrap.qs{1} = G0o.qs{2} /\ Wrap.sk{1} = G0o.sk{2} ==>
-    ={glob G,glob H, res} /\ Wrap.qs{1} = G0o.qs{2} /\ Wrap.sk{1} = G0o.sk{2}].
-proof.
-fun; inline PSS''(G,H).sign CorrectG.call1;
-wp 12 8; eqobs_in.
-qed.
-
-local equiv PSS''_G0_init: Wrap(PSS''(G,H)).init ~ G0o(G,H).init:
-  true ==>
-  ={glob G, glob H, res} /\
-  Wrap.qs{1} = G0o.qs{2} /\
-  Wrap.pk{1} = G0o.pk{2} /\
-  Wrap.sk{1} = G0o.sk{2} /\
-  G0o.pk{2} = res{2}.
-proof.
-fun; inline PSS''(G,H).init PSS''(G,H).keygen PSS(G,H).init.
-wp; rnd; wp.
-seq 2 2: (={glob G, glob H})=> //.
-call (_: true ==> ={glob H})=> //;
-  first by fun (true).
-call (_: true ==> ={glob G})=> //;
-  first by fun (true).
-qed.
-
-(** We really *really* **really** want to be able to prove PSS_G0
-    in one step, which requires being able to use correct_G to discharge
-    an objective of the form:
-
-
-    pre: x{1} = w{2} /\ x0{1} = w{2}
-
-    g = G.o(x)                       (1)  g = G.o(x)
-    g' = G.o(x0)                     (2)
-
-    post: (g,g'){1} = (g,g){2} *)
-local equiv PSS''_G0:
-  EF_CMA(Wrap(PSS''(G,H)),Adv(G,H)).main ~ G0(G,H,G0o(G,H),Adv(G,H)).main:
-    ={glob Adv} ==> ={res}.
-proof.
-fun;
-call PSS''_G0_fresh.
-seq 2 2: (={glob G, glob H, m, s} /\
-          Wrap.qs{1} = G0o.qs{2} /\
-          Wrap.pk{1} = G0o.pk{2} /\
-          G0o.pk{2} = pk{2}).
-  call (_: ={glob G, glob H} /\
-           Wrap.qs{1} = G0o.qs{2} /\
-           Wrap.pk{1} = G0o.pk{2} /\
-           Wrap.sk{1} = G0o.sk{2}).
-    by conseq* PSS''_G0_sign.
-    by conseq* (_: ={glob H, x} ==> ={glob H, res})=> //; fun (true).
-    by conseq* (_: ={glob G, x} ==> ={glob G, res})=> //; fun (true).
-  by call PSS''_G0_init.
-inline Wrap(PSS''(G,H)).verify PSS''(G,H).verify CorrectG.call1.
-conseq * (_: ={glob H, glob G, m, s} /\ Wrap.pk{1} = G0o.pk{2} /\ G0o.pk{2} = pk{2} ==>
-             ={glob H, glob G, forged} /\ Wrap.pk{1} = G0o.pk{2})=> //.
-wp.
-call (_: true).
-wp.
-call (_: true).
-by wp; skip.
-qed.
-
-lemma PSS_G0_sectioned &m:
-  Pr[EF_CMA(Wrap(PSS(G,H)),Adv(G,H)).main() @ &m: res] = Pr[G0(G,H,G0o(G,H),Adv(G,H)).main() @ &m: res].
-proof.
-cut ->: Pr[EF_CMA(Wrap(PSS(G,H)),Adv(G,H)).main() @ &m: res] =
-          Pr[EF_CMA(Wrap(PSS'(G,H)),Adv(G,H)).main() @ &m: res]
-  by by equiv_deno PSS_PSS'.
-cut ->: Pr[EF_CMA(Wrap(PSS'(G,H)),Adv(G,H)).main() @ &m: res] =
-          Pr[EF_CMA(Wrap(PSS''(G,H)),Adv(G,H)).main() @ &m: res]
-  by by equiv_deno PSS'_PSS''.
-by equiv_deno PSS''_G0.
-qed.
-end section.
-
-lemma PSS_G0 &m:
-  Pr[EF_CMA(Wrap(PSS(G,H)),Adv(G,H)).main() @ &m: res] = Pr[G0(G,H,G0o(G,H),Adv(G,H)).main() @ &m: res].
-proof.
-apply (PSS_G0_sectioned G H _ _ &m)=> //.
-  by apply AdvL.
-  by apply Gt.ROM.correct_RO.
-qed.
-end section.
-
-(** Second transition: Split H to distinguish queries made directly
-    by the adversary from those made during the execution of an oracle. *)
-clone import RandomOracle as Ht' with
-  type from <- (message * salt),
-  type to <- htag,
-  op dsample <- sample_htag.
-
-require import Map.
-module Hstate = {
-  var qs: (message * salt) set
-  var m: ((message * salt) * bool,htag) map
-}.
-
-module H':Ht'.Oracle = {
-  fun init(): unit = {
-    Hstate.m = Map.empty;
-    Hstate.qs = FSet.empty;
-  }
-
-  fun o(x:message * salt): htag = {
-    Hstate.qs = add x Hstate.qs;
-    if (!mem x Hstate.qs) Hstate.m.[(x,false)] = $sample_htag;
-    return proj Hstate.m.[proj (find (lambda a b, fst a = x) Hstate.m)];
-  }
-}.
-
-module Ha':Ht'.Oracle = {
-  fun init(): unit = {
-    Hstate.m = Map.empty;
-    Hstate.qs = FSet.empty;
-  }
-
-  fun o(x:message * salt): htag = {
-    Hstate.qs = add x Hstate.qs;
-    if (!mem x Hstate.qs) Hstate.m.[(x,true)] = $sample_htag;
-    return proj Hstate.m.[proj (find (lambda a b, fst a = x) Hstate.m)];
-  }
-}.
-
-module G1o(G:Gt.Oracle,H:Ht'.Oracle) = {
-  var pk:pkey
-  var sk:skey
-
-  var qs:message set
-
-  fun init(): pkey = {
-    G.init();
-    H.init();
-    qs = FSet.empty;
-    (pk,sk) = $keypairs;
+    Mem.init(pk,sk);
     return pk;
   }
 
@@ -612,7 +255,7 @@ module G1o(G:Gt.Oracle,H:Ht'.Oracle) = {
   }
 }.
 
-module G1(G:Gt.Oracle,H:Ht.Oracle,O:PartialOracles,A:AdvCMA) = {
+module GGen(H:Ht.Oracle,O:PartialOracles,A:AdvCMA) = {
   module A = A(O)
 
   fun main(): bool = {
@@ -641,7 +284,7 @@ module G1(G:Gt.Oracle,H:Ht.Oracle,O:PartialOracles,A:AdvCMA) = {
     g = G.o(w);
     rMask  = Salt.from_bits (sub (to_bits g) 0 k0);
     r = rMask ^ maskedR;
-    w'  = H.o(m || to_bits r);
+    w'  = H.o((m,r));
     gamma'  = G2Tag.from_bits (sub (to_bits g) k0 kg2);
     forged =  w = w' /\ gamma = gamma' /\ !forged;
 
@@ -650,23 +293,438 @@ module G1(G:Gt.Oracle,H:Ht.Oracle,O:PartialOracles,A:AdvCMA) = {
   }
 }.
 
-(* PROOF GOES HERE *)
+module G0 = GGen(H,SGen(H)).
 
+(** H Oracle for G1 *)
+op bool_nu: int -> bool distr.
+axiom mu_bool_nu N p:
+  2^(k - 1) <= N < 2^k =>
+  mu (bool_nu N) p =
+    (N%r - (2^(k-1))%r / N%r) * charfun p true + ((2^(k - 1))%r / N%r) * charfun p false.
 
-(* We bound the probability, for all lossless
-   adversary A of type CMA_2RO of
-   PSS_CMA(A(G',H')).main returning true. *)
-section.
-declare module Adv:CMA_2RO.
-declare module I:Inverter.
-local lemma local_conclusion &m:
-  Pr[EF_CMA(Wrap(PSS(G,H)),Adv(G,H)).main() @ &m: res] <= Pr[RSA.OW(I).main() @ &m: res].
-admit.
-qed.
+module H1: Ht.Oracle = {
+  var bad:bool
 
-lemma conclusion &m: exists (I<:Inverter),
-  Pr[EF_CMA(Wrap(PSS(G,H)),Adv(G,H)).main() @ &m: res] <= Pr[RSA.OW(I).main() @ &m: res].
+  fun init(): unit = {
+    H.init();
+    bad = false;
+  }
+
+  fun o(x:message * salt): htag = {
+    var b:bool = true;
+    var i:int = 0;
+    var w:htag;
+    w = $sample_htag;
+    if (!in_dom x H.m)
+    {
+      while (i < kg2 && b)
+      {
+        b = $bool_nu Mem.n;
+        i = i + 1;
+        if (!b)
+          H.m.[x] = w;
+      }
+    }
+    bad = bad \/ b;
+    return proj H.m.[x];
+  }
+}.
+
+module G1 = GGen(H1,SGen(H1)).
+
+(** Proof is up to bad with BAD = (b = true) in final memory *)
+lemma equiv_G0_G1 (A <: CMA_2RO):
+  equiv [G0(A(G,H)).main ~ G1(A(G,H1)).main: ={glob A} ==> !H1.bad{2} => ={res}].
+admit. qed.
+
+lemma G0_G1 (A <: CMA_2RO) &m:
+  Pr[G0(A(G,H)).main() @ &m: res] <= Pr[G1(A(G,H1)).main() @ &m: res] + Pr[G1(A(G,H1)).main() @ &m: H1.bad].
 proof.
-exists I; apply (local_conclusion &m).
+apply (Trans _ Pr[G1(A(G,H1)).main() @ &m: res \/ H1.bad] _).
+equiv_deno (equiv_G0_G1 A)=> //; smt.
+rewrite Pr mu_or; smt.
 qed.
-end section.
+
+(** Maybe we need to fix the event to add a bound on the number of queries in the game *)
+lemma Bad1 (A <: CMA_2RO) &m:
+  Pr[G1(A(G,H1)).main() @ &m: H1.bad] <= (qS + qH)%r/(2^kg2)%r.
+admit. qed.
+
+(** G2 *)
+module H2: Ht.Oracle = {
+  fun init(): unit = {
+    H.init();
+  }
+
+  fun o(x:message * salt): htag = {
+    var b:bool = true;
+    var i:int = 0;
+    var w:htag;
+    if (!in_dom x H.m)
+    {
+      while (i < kg2 && b)
+      {
+        b = $bool_nu Mem.n;
+        w = $sample_htag;
+        i = i + 1;
+        if (!b)
+          H.m.[x] = w;
+      }
+    }
+    return proj H.m.[x];
+  }
+}.
+
+module G2 = GGen(H2,SGen(H2)).
+
+equiv equiv_G1_G2 (A <: CMA_2RO):
+  G1(A(G,H1)).main ~ G2(A(G,H2)).main: ={glob A} ==> ={res}.
+admit. 
+(** Proof goes by eager (rule for while in figure 3 in the ITP paper) *)
+(* We may need to modify H2 so that it samples an initial (useless) value for w *)
+(* Swapping statement is "if (b) w = $sample_htag;" *)
+qed.
+
+(** G3 *)
+module H3: Ht.Oracle = {
+  fun init(): unit = {
+    H.init();
+  }
+
+  fun o (x:message * salt): htag = {
+    var b:bool = true;
+    var i:int = 0;
+    var w:htag;
+    var st:gtag;
+    if (!in_dom x H.m)
+    {
+      while (i < kg2 && b)
+      {
+        b = $bool_nu Mem.n;
+        w = $sample_htag;
+        i = i + 1;
+        if (!b)
+        {
+          H.m.[x] = w;
+          st = G.o(w);
+        }
+      }
+    }
+    return proj H.m.[x];
+  }
+}.
+
+module G3 = GGen(H3,SGen(H3)).
+
+(** The proof is by two applications of the general eager-lazy transition for G:
+      - first, we eagerly sample G,
+      - then, we lazily sample it again (with some calls happening in H).        *)
+equiv equiv_G2_G3 (A <: CMA_2RO):
+  G2(A(G,H2)).main ~ G3(A(G,H3)).main: ={glob A} ==> ={res}.
+admit. qed.
+
+(** G4 *)
+module H4: Ht.Oracle = {
+  var bad:bool
+
+  fun init(): unit = {
+    H.init();
+    bad = false;
+  }
+
+  fun o (x:message * salt): htag = {
+    var b:bool = true;
+    var i:int = 0;
+    var w:htag;
+    var st:gtag;
+    if (!in_dom x H.m)
+    {
+      while (i < kg2 && b)
+      {
+        b = $bool_nu Mem.n;
+        w = $sample_htag;
+        st = $sample_gtag;
+        i = i + 1;
+        if (!b)
+        {
+          H.m.[x] = w;
+          bad = bad \/ in_dom w G.m;
+          G.m.[w] = st ^ (GTag.from_bits (to_bits (snd x) || zeros (kg - k0)));
+        }
+      }
+    }
+    return proj H.m.[x];
+  }
+}.
+
+module G4 = GGen(H4,SGen(H4)).
+
+(** Proof is up to failure *)
+equiv equiv_G3_G4 (A <: CMA_2RO):
+  G3(A(G,H3)).main ~ G4(A(G,H4)).main: ={glob A} ==> !H4.bad{2} => ={res}.
+admit. qed.
+
+lemma G3_G4 (A <: CMA_2RO) &m:
+  Pr[G3(A(G,H3)).main() @ &m: res] <= Pr[G4(A(G,H4)).main() @ &m: res] + Pr[G4(A(G,H4)).main() @ &m: H4.bad].
+proof.
+apply (Trans _ Pr[G4(A(G,H4)).main() @ &m: res \/ H4.bad]).
+equiv_deno (equiv_G3_G4 A)=> //; smt.
+rewrite Pr mu_or; smt.
+qed.
+
+(* We will need the invariant that `|dom G.m| <= qG *)
+lemma Bad4 (A <: CMA_2RO) &m:
+  Pr[G4(A(G,H4)).main() @ &m: H4.bad] <= (qS + qH)%r * (qG + qS + qH)%r/(2^k1)%r.
+admit. qed.
+
+(** Splitting the random oracle *)
+module type SplitOracle = {
+  fun init(): unit
+  fun o(c:bool,x:message * salt):htag
+}.
+
+module Hs(H:SplitOracle): Ht.Oracle = {
+  fun init(): unit = {
+    H.init();
+  }
+
+  fun o(x:message * salt): htag = {
+    var r:htag;
+    r = H.o(false,x);
+    return r;
+  }
+}.
+
+module Ha(H:SplitOracle): Ht.Oracle = {
+  fun init(): unit = {
+    H.init();
+  }
+
+  fun o(x:message * salt): htag = {
+    var r:htag;
+    r = H.o(true,x);
+    return r;
+  }
+}.
+
+(** G5 *)
+module H5: SplitOracle = {
+  var bad:bool
+  var m:(message * salt,htag * bool) map
+
+  fun init(): unit = {
+    m = Map.empty;
+  }
+
+  fun o(c:bool,x:message * salt): htag = {
+    var b:bool = true;
+    var i:int = 0;
+    var w:htag;
+    var st:gtag;
+    if (!in_dom x H.m)
+    {
+      while (i < kg2 && b)
+      {
+        b = $bool_nu Mem.n;
+        w = $sample_htag;
+        st = $sample_gtag;
+        i = i + 1;
+        if (!b)
+        {
+          m.[x] = (w,c);
+          G.m.[w] = st ^ (GTag.from_bits (to_bits (snd x) || zeros (kg - k0)));
+        }
+      }
+    }
+    else
+    {
+      if (!c /\ snd (proj H5.m.[x]))
+      {
+        bad = true;
+        m.[x] = (HTag.zeros,c);
+      }
+    }
+    return fst (proj m.[x]);
+  }
+}.
+
+module G5 = GGen(Hs(H5),SGen(Hs(H5))).
+
+equiv equiv_G4_G5 (A <: CMA_2RO):
+  G4(A(G,H4)).main ~ G5(A(G,Ha(H5))).main: ={glob A} ==> !H5.bad{2} => ={res}.
+admit. qed.
+
+lemma Bad5 (A <: CMA_2RO) &m:
+  Pr[G5(A(G,Ha(H5))).main() @ &m: H5.bad] <= qS%r * (qS + qH)%r/(2^k0)%r.
+admit. qed.
+
+(** G6 *)
+module H6: SplitOracle = {
+  var bad:bool
+  var m:(message * salt,htag * bool * signature) map
+
+  fun init(): unit = {
+    m = Map.empty;
+  }
+
+  fun o(c:bool,x:message * salt): htag = {
+    var b:bool = true;
+    var i:int = 0;
+    var w:htag;
+    var st:gtag;
+    var z, u:signature;
+
+    if (!in_dom x H.m)
+    {
+      while (i < kg2 && b)
+      {
+        b = $bool_nu Mem.n;
+        w = $sample_htag;
+        st = $sample_gtag;
+        z = Signature.from_bits (if b then ones 1 else zeros 1 || to_bits w || to_bits st);
+        u = if c then (Mem.xstar * finv Mem.sk  z) Mem.pk else finv Mem.sk z;
+        i = i + 1;
+        if (!b)
+        {
+          m.[x] = (w,c,u);
+          G.m.[w] = st ^ (GTag.from_bits (to_bits (snd x) || zeros (kg - k0)));
+        }
+      }
+    }
+    else
+    {
+      bad = true;
+      if (!c) m.[x] = (HTag.zeros,c,Signature.zeros);
+    }
+    return proj H.m.[x];
+  }
+}.
+
+module G6 = GGen(Hs(H6),SGen(Hs(H6))).
+
+(** G7: No longer using sk to simulate the oracles *)
+module H7: SplitOracle = {
+  var bad:bool
+  var m:(message * salt,htag * bool * signature) map
+
+  fun init(): unit = {
+    m = Map.empty;
+  }
+
+  fun o(c:bool,x:message * salt): htag = {
+    var b:bool = true;
+    var i:int = 0;
+    var w:htag;
+    var st:gtag;
+    var z, u:signature;
+
+    if (!in_dom x H.m)
+    {
+      while (i < kg2 && b)
+      {
+        u = $sample_plain;
+        z = if c then (f Mem.pk Mem.xstar * f Mem.pk u) Mem.pk else f Mem.pk u;
+        b = (sub (to_bits z) 0 1 = ones 1);
+        w = HTag.from_bits (sub (to_bits z) 1 k1);
+        st = GTag.from_bits (sub (to_bits z) (k1 + 1) (kg));
+        i = i + 1;
+        if (!b)
+        {
+          m.[x] = (w,c,u);
+          G.m.[w] = st ^ (GTag.from_bits (to_bits (snd x) || zeros (kg - k0)));
+        }
+      }
+    }
+    else
+    {
+      bad = true;
+      if (!c) m.[x] = (HTag.zeros,c,Signature.zeros);
+    }
+    return (lambda abc, let (a,b,c) = abc in a) (proj m.[x]);
+  }
+}.
+
+module G7 = GGen(Hs(H7),SGen(Hs(H7))).
+
+(** Inverter *)
+module I(A:CMA_2RO): Inverter = {
+  var pk:pkey
+  var n:int
+  var ystar:signature
+
+  module H = {
+    var m:(message * salt,htag * bool * signature) map
+
+    fun init(): unit = { }
+
+    fun o(c:bool,x:message * salt): htag = {
+      var b:bool = true;
+      var i:int = 0;
+      var w:htag;
+      var st:gtag;
+      var z, u:signature;
+
+      if (!in_dom x H.m)
+      {
+        while (i < kg2 && b)
+        {
+          u = $sample_plain;
+          z = if c then (ystar * f pk u) pk else f pk u;
+          b = (sub (to_bits z) 0 1 = ones 1);
+          w = HTag.from_bits (sub (to_bits z) 1 k1);
+          st = GTag.from_bits (sub (to_bits z) (k1 + 1) (kg));
+          i = i + 1;
+          if (!b)
+          {
+            m.[x] = (w,c,u);
+            G.m.[w] = st ^ (GTag.from_bits (to_bits (snd x) || zeros (kg - k0)));
+          }
+        }
+      }
+      else
+      {
+        if (!c) m.[x] = (HTag.zeros,c,Signature.zeros);
+      }
+      return (lambda abc, let (a,b,c) = abc in a) (proj m.[x]);
+    }
+  }     
+
+  module IOracles = {
+    var qs:message set
+
+    fun init(): unit = {
+      qs = FSet.empty;
+      H.m = Map.empty;
+    }
+
+    fun sign(m:message): signature = {
+      var r:salt;
+      var w:htag;
+      r = $sample_salt;
+      w = H.o(false,(m,r));
+      return (lambda abc, let (a,b,c) = abc in c) (proj H.m.[(m,r)]);
+    }
+
+    fun fresh(m:message): bool = {
+      return !mem m qs;
+    }
+  }
+
+  module A = A(G,Ha(H),IOracles)
+
+  fun inverter(pk:pkey,y:signature): signature = {
+    var m:message;
+    var s:signature;
+
+    I.pk = pk;
+    n = 3;
+    ystar = y;
+    (m,s) = A.forge(pk);
+
+    return s;
+  }
+}.
+
+equiv equiv_G7_OW (A<:CMA_2RO):
+  G7(A(G,Ha(H7))).main ~ OW(I(A)).main: ={glob A} ==> ={res}.
+admit. qed.
